Sweet solution for enumerator termination measure

src/Actions/Actions.dfy
@@ -23,7 +23,7 @@ module Actions {
         && CanProduce(consumed, produced)
       decreases Repr, 0
     
-    ghost predicate CanConsume(consumed: seq<T>, produced: seq<R>, nextIn: T)
+    ghost predicate CanConsume(consumed: seq<T>, produced: seq<R>, next: T)
       requires CanProduce(consumed, produced)
 
     ghost predicate CanProduce(consumed: seq<T>, produced: seq<R>)
@@ -41,15 +41,18 @@ module Actions {
       requires Valid()
       requires CanConsume(consumed, produced, t)
       modifies Repr
+      decreases Repr
       ensures Valid()
-      // TODO: Might be too limiting, could have a similar predicate for valid Repr changes.
-      // At least this is necessary most of the time if you want to invoke an action multiple times,
-      // But won't be true in general (e.g. an aggregator that has to allocate more storage).
+      // TODO: Will cause trouble when composing, see FilteredEnumerator in Enumerators.dfy
+      // ensures fresh(Repr - old(Repr))
+      // TODO: Not compatible with all actions
       ensures Repr <= old(Repr)
       ensures consumed == old(consumed) + [t]
       ensures produced == old(produced) + [r]
       ensures CanProduce(consumed, produced)
   }
+
+  // Common action invariants
 
   ghost predicate OnlyProduces<T(!new), R(!new)>(i: Action<T, R>, c: R) {
     forall consumed: seq<T>, toProduce: seq<R> :: 
@@ -60,11 +63,64 @@ module Actions {
     forall i, j | 0 <= i < j < |s| :: s[i] == c ==> s[j] == c
   }
 
-  ghost predicate ProducesTerminatedBy<T(!new), R(!new)>(i: Action<T, R>, c: R) {
-    forall consumed: seq<T>, toProduce: seq<R> ::
-      i.CanProduce(consumed, toProduce) ==> TerminatedBy(toProduce, c)
+  ghost predicate TerminatedByBeyond<T>(s: seq<T>, c: T, n: nat) {
+    forall i | n <= i < |s| :: s[i] == c
   }
 
+  function Enumerated<T>(produced: seq<Option<T>>): seq<T> {
+    if |produced| == 0 || produced[0].None? then
+      []
+    else
+      [produced[0].value] + Enumerated(produced[1..])
+  }
+
+  lemma TerminatedByBoundsEnumerated<T>(s: seq<Option<T>>, n: nat) 
+    requires TerminatedByBeyond(s, None, n)
+    ensures |Enumerated(s)| <= n
+  {
+    if |s| == 0 || s[0].None? {
+    } else {
+      TerminatedByBoundsEnumerated(s[1..], n - 1);
+    }
+  }
+
+  ghost function ProducedForEnumerator<T>(s: seq<T>, n: nat): seq<Option<T>> {
+    var before := Math.Min(|s|, n);
+    var after := Math.Max(|s|, n);
+    Seq.Map(x => Some(x), s[..before]) + Seq.Repeat(None, after - before)
+  }
+
+  ghost predicate EnumeratesAtMost<T(!new)>(e: Action<(), Option<T>>, n: nat) {
+    forall consumed: seq<()>, toProduce: seq<Option<T>> ::
+      e.CanProduce(consumed, toProduce) ==> |Enumerated(toProduce)| <= n
+  }
+
+  
+
+  ghost predicate ProducesTerminatedBy<T(!new), R(!new)>(i: Action<T, R>, c: R, n: nat) {
+    forall consumed: seq<T>, toProduce: seq<R> ::
+      i.CanProduce(consumed, toProduce) ==> TerminatedByBeyond(toProduce, c, n)
+  }
+
+  ghost predicate ConsumesAnything<T(!new)>(a: Action<(), Option<T>>) {
+    forall consumed, produced, next | a.CanProduce(consumed, produced) :: a.CanConsume(consumed, produced, next)
+  }
+
+  ghost predicate IsEnumerator<T(!new)>(a: Action<(), Option<T>>) {
+    ConsumesAnything(a) && exists n :: ProducesTerminatedBy(a, None, n)
+  }
+
+  ghost function EnumerationDecreases<T(!new)>(a: Action<(), Option<T>>): nat
+    requires a.Valid()
+    reads a.Repr
+    requires IsEnumerator(a)
+  {
+    var limit: nat :| ProducesTerminatedBy(a, None, limit);
+    TerminatedByBoundsEnumerated(a.produced, limit);
+    limit - |Enumerated(a.produced)|
+  }
+
+  // Potentially infinite enumerator
   type IEnumerator<T> = Action<(), T> 
 
   class SeqIEnumerator<T> extends Action<(), T> {
@@ -110,6 +166,7 @@ module Actions {
       requires Valid()
       requires CanConsume(consumed, produced, t)
       modifies Repr
+      decreases Repr
       ensures Valid()
       ensures Repr <= old(Repr)
       ensures consumed == old(consumed) + [t]
@@ -123,44 +180,219 @@ module Actions {
     }
   }
 
-  method Main() {
-    var e: Action<(), int> := new SeqIEnumerator([1, 2, 3, 4, 5]);
-    var x := e.Invoke(());
-    assert e.produced == [1];
-    x := e.Invoke(());
-    assert e.produced == [1, 2];
-    x := e.Invoke(());
-    assert e.produced == [1, 2, 3];
-    x := e.Invoke(());
-    assert e.produced == [1, 2, 3, 4];
-    x := e.Invoke(());
-    assert e.produced == [1, 2, 3, 4, 5];
+  class Filter<T(!new)> extends Action<(), Option<T>> {
+
+    const wrapped: Action<(), Option<T>>
+      
+    // TODO: Can we support --> or ~>?
+    const filter: T -> bool
+
+    ghost predicate Valid() 
+      reads this, Repr 
+      ensures Valid() ==> this in Repr 
+      ensures Valid() ==> 
+        && CanProduce(consumed, produced)
+      decreases Repr, 0
+    {
+      && this in Repr
+      && ValidComponent(wrapped)
+      && IsEnumerator(wrapped)
+      && CanProduce(consumed, produced)
+    }
+
+    constructor(filter: T -> bool, wrapped: Action<(), Option<T>>) 
+      requires wrapped.Valid()
+      requires IsEnumerator(wrapped)
+      requires wrapped.consumed == [] && wrapped.produced == []
+      ensures Valid()
+    { 
+      this.filter := filter;
+      this.wrapped := wrapped;
+
+      consumed := [];
+      produced := [];
+      Repr := {this} + wrapped.Repr;
+    }
+
+    ghost predicate CanConsume(consumed: seq<()>, produced: seq<Option<T>>, next: ()) {
+      true
+    }
+    ghost predicate CanProduce(consumed: seq<()>, produced: seq<Option<T>>) {
+      exists producedByWrapped: seq<Option<T>> ::
+        && wrapped.CanProduce(Seq.Repeat((), |producedByWrapped|), producedByWrapped)
+        && Enumerated(produced) == Seq.Filter(filter, Enumerated(producedByWrapped))
+    }
+
+    method Invoke(t: ()) returns (r: Option<T>) 
+      requires Valid()
+      requires CanConsume(consumed, produced, t)
+      modifies Repr
+      decreases Repr
+      ensures Valid()
+      ensures Repr <= old(Repr)
+      ensures consumed == old(consumed) + [t]
+      ensures produced == old(produced) + [r]
+      ensures CanProduce(consumed, produced)
+    {
+      assert Enumerated(produced) == Seq.Filter(filter, Enumerated(wrapped.produced));
+      r := wrapped.Invoke(());
+      while r.Some? && !filter(r.value)
+        invariant Valid()
+        invariant Enumerated(produced) == Seq.Filter(filter, Enumerated(wrapped.produced))
+        decreases EnumerationDecreases(wrapped)
+      {
+        r := wrapped.Invoke(());
+      }
+
+      Update(t, r);
+    }
   }
 
-  // TODO: Not strong enough, could still be infinite. exists n | terminated beyond n?
-  // TODO: How to provide decreases clause for loops etc?
-  type Enumerator<T(!new)> = a: Action<(), Option<T>> | ProducesTerminatedBy(a, None) witness *
+  // class Compose<T, V(!new), R> extends Action<T, R> {
 
-  function Enumerated<T>(produced: seq<Option<T>>): seq<T> {
-    if |produced| == 0 || produced[0].None? then
-      []
-    else
-      [produced[0].value] + Enumerated(produced[1..])
-  }
+  //   const first: Action<T, V>
+  //   const second: Action<V, R>
 
-  ghost function ProducedForEnumerator<T>(s: seq<T>, n: nat): seq<Option<T>> {
-    var before := Math.Min(|s|, n);
-    var after := Math.Max(|s|, n);
-    Seq.Map(x => Some(x), s[..before]) + Seq.Repeat(None, after - before)
-  }
+  //   ghost predicate Valid() 
+  //     reads this, Repr 
+  //     ensures Valid() ==> this in Repr 
+  //     ensures Valid() ==> 
+  //       && CanProduce(consumed, produced)
+  //     decreases Repr, 0
+  //   {
+  //     && this in Repr
+  //     && ValidComponent(first)
+  //     && ValidComponent(second)
+  //     && CanProduce(consumed, produced)
+  //   }
 
-  ghost predicate EnumeratesAtMost<T(!new)>(e: Enumerator<T>, n: nat) {
-    forall consumed: seq<()>, toProduce: seq<Option<T>> ::
-      e.CanProduce(consumed, toProduce) ==> |Enumerated(toProduce)| <= n
-  }
+  //   constructor(second: Action<V, R>, first: Action<T, V>) 
+  //     requires first.Valid()
+  //     requires second.Valid()
+  //     requires first.Repr !! second.Repr
+  //     requires first.CanProduce([], [])
+  //     requires second.CanProduce([], [])
+  //     ensures Valid()
+  //     ensures produced == []
+  //   { 
+  //     this.first := first;
+  //     this.second := second;
+
+  //     consumed := [];
+  //     produced := [];
+  //     Repr := {this} + first.Repr + second.Repr;
+  //   }
+
+  //   ghost predicate CanConsume(consumed: seq<T>, produced: seq<R>, next: T) {
+  //     exists vs: seq<V> :: 
+  //       && first.CanProduce(consumed, vs)
+  //       && first.CanConsume(consumed, vs, next)
+  //   }
+  //   ghost predicate CanProduce(consumed: seq<T>, produced: seq<R>) {
+  //     exists vs: seq<V> :: first.CanProduce(consumed, vs) && second.CanProduce(vs, produced)
+  //   }
+
+  //   method Invoke(t: T) returns (r: R) 
+  //     requires Valid()
+  //     requires CanConsume(consumed, produced, t)
+  //     modifies Repr
+  //     decreases Repr
+  //     ensures Valid()
+  //     ensures Repr <= old(Repr)
+  //     ensures consumed == old(consumed) + [t]
+  //     ensures produced == old(produced) + [r]
+  //     ensures CanProduce(consumed, produced)
+  //   {
+  //     var v := first.Invoke(t);
+  //     r := second.Invoke(v);
+
+  //     Update(t, r);
+  //   }
+
+  // }
 
   type IAggregator<T> = Action<T, ()>
-  type Aggregator<T(!new)> = a: Action<T, bool>  | ProducesTerminatedBy(a, false) witness *
+  type Aggregator<T(!new)> = a: Action<T, bool> | exists n :: ProducesTerminatedBy(a, false, n) witness *
+
+  class ArrayAggregator<T(0)> extends Action<T, ()> {
+
+    var storage: array<T>
+    var index: nat
+
+    ghost predicate Valid() 
+      reads this, Repr 
+      ensures Valid() ==> this in Repr 
+      ensures Valid() ==> 
+        && CanProduce(consumed, produced)
+      decreases Repr, 0
+    {
+      && this in Repr
+      && storage in Repr
+      && 0 < storage.Length
+      && 0 <= index <= storage.Length
+      && consumed == storage[..index]
+      && produced == Seq.Repeat((), |consumed|)
+    }
+
+    constructor() 
+      ensures Valid()
+      ensures fresh(Repr - {this})
+      ensures produced == []
+    {
+      index := 0;
+      storage := new T[10];
+
+      consumed := [];
+      produced := [];
+      Repr := {this, storage};
+    }
+
+    ghost predicate CanConsume(consumed: seq<T>, produced: seq<()>, next: T) {
+      true
+    }
+    ghost predicate CanProduce(consumed: seq<T>, produced: seq<()>) {
+      produced == Seq.Repeat((), |consumed|)
+    }
+
+    twostate predicate ValidReprChange(before: set<object>, after: set<object>) {
+      fresh(after - before)
+    }
+
+    method Invoke(t: T) returns (r: ()) 
+      requires Valid()
+      requires CanConsume(consumed, produced, t)
+      modifies Repr
+      decreases Repr
+      ensures Valid()
+      ensures fresh(Repr - old(Repr))
+      ensures consumed == old(consumed) + [t]
+      ensures produced == old(produced) + [r]
+      ensures CanProduce(consumed, produced)
+    {
+      if index == storage.Length {
+        var newStorage := new T[storage.Length * 2];
+        forall i | 0 <= i < index {
+          newStorage[i] := storage[i];
+        }
+        storage := newStorage;
+
+        Repr := {this, storage};
+      }
+      storage[index] := t;
+      index := index + 1;
+
+      r := ();
+      Update(t, r);
+    }
+
+    function Values(): seq<T>
+      requires Valid()
+      reads Repr
+      ensures Values() == consumed
+    {
+      storage[..index]
+    }
+  }
 
   // class SeqEnumerator<T> extends Action<(), Option<T>> {
 
@@ -214,4 +446,25 @@ module Actions {
 
 
 
+  method Main() {
+    var e: Action<(), int> := new SeqIEnumerator([1, 2, 3, 4, 5]);
+    var x := e.Invoke(());
+    assert e.produced == [1];
+    x := e.Invoke(());
+    assert e.produced == [1, 2];
+    x := e.Invoke(());
+    assert e.produced == [1, 2, 3];
+    x := e.Invoke(());
+    assert e.produced == [1, 2, 3, 4];
+    x := e.Invoke(());
+    assert e.produced == [1, 2, 3, 4, 5];
+
+    var a := new ArrayAggregator();
+    var _ := a.Invoke(1);
+    var _ := a.Invoke(2);
+    var _ := a.Invoke(3);
+    var _ := a.Invoke(4);
+    var _ := a.Invoke(5);
+    assert a.Values() == [1, 2, 3, 4, 5];
+  }
 }
